Day 6

problems/6/Problem6.dfy
@@ -1,9 +1,142 @@
+include "../../parser/split.dfy"
 module Problem6 {
-    method problem6_1(input: string) returns (x: int) {
-        return 3;
+    import opened Split
+    import opened Std.Collections.Seq
+    method parseInput(input: string) returns (obstacles: set<(int, int)>, start: (int, int), dim: (nat, nat)) 
+    {
+        start := (0, 0);
+        obstacles := {};
+        var lines := splitOnBreak(input);
+        for y := 0 to |lines| 
+        {
+            if lines[y] != "" {
+                for x := 0 to |lines[y]| 
+                {
+                    if lines[y][x] == '#' {
+                        obstacles := obstacles + {(x, y)};
+                    }else if lines[y][x] == '^' {
+                        start := (x, y);
+                    }
+                }
+            }
+        }
+        expect |lines| > 0;
+        dim := (|lines[0]|, |lines|-1);
     }
 
-    method problem6_2(input: string) returns (x: int) {
-        return 4;
+    datatype Direction = Up | Down | Left | Right
+    function TurnRight(d: Direction): Direction 
+    {
+        match d {
+            case Up => Right
+            case Down => Left
+            case Left => Up
+            case Right => Down
+        }
+    }
+
+    function step(d: Direction, p: (int, int)): (int, int) 
+    {
+        match d {
+            case Up => (p.0, p.1 - 1)
+            case Down => (p.0, p.1 + 1)
+            case Left => (p.0 - 1, p.1)
+            case Right => (p.0 + 1, p.1)
+        }
+    }
+
+    predicate InBounds(p: (int, int), dim: (nat, nat)) 
+    {
+        0 <= p.0 < dim.0 && 0 <= p.1 < dim.1
+    }
+
+    method IsLoop(start: (int, int), obstacles: set<(int, int)>, dim: (nat, nat)) returns (b: bool)
+        decreases *
+    {
+        var visited: set<(Direction, (int, int))> := {(Up, start)};
+        var curr := start;
+        var dir := Up;
+        while InBounds(curr, dim)
+            decreases *
+        {
+            visited := visited + {(dir, curr)};
+            var next := step(dir, curr);
+            while next in obstacles 
+                decreases *
+            {
+                dir := TurnRight(dir);
+                next := step(dir, curr);
+            }
+            if (dir, next) in visited {
+                b := true;
+                return;
+            }
+            curr := next;
+        }
+        b := false;
+    }
+
+    method problem6_1(input: string) returns (x: int) 
+        decreases *
+    {
+        var obstacles, start, dim := parseInput(input);
+        x := 0;
+        var visited := {start};
+        var curr := start;
+        var dir := Up;
+        while InBounds(curr, dim)
+            decreases *
+        {
+            visited := visited + {curr};
+            var next := step(dir, curr);
+            while next in obstacles 
+                decreases *
+            {
+                dir := TurnRight(dir);
+                next := step(dir, curr);
+            }
+            curr := next;
+        }
+        x := |visited|;
+    }
+
+    method problem6_2(input: string) returns (x: int) 
+        decreases *
+    {
+        var obstacles, start, dim := parseInput(input);
+        var visited := {start};
+        var curr := start;
+        var dir := Up;
+        x := 0;
+        while InBounds(curr, dim)
+            decreases *
+        {
+            visited := visited + {curr};
+            var next := step(dir, curr);
+            while next in obstacles 
+                decreases *
+            {
+                dir := TurnRight(dir);
+                next := step(dir, curr);
+            }
+            curr := next;
+        }
+        var vs := SetToSeq(visited);
+        var newobs: set<(int, int)> := {};
+        while vs != []
+            decreases |vs|
+        {
+            var curr := vs[0];
+            if curr == start {
+                vs := vs[1..];
+                continue;
+            }
+            var loop := IsLoop(start, obstacles+{curr}, dim);
+            if loop {
+                newobs := newobs + {curr};
+            }
+            vs := vs[1..];
+        }
+        x := |newobs|;
     }
 }
